theories/iris/examples/stack/function/pop.v
@@ -4,7 +4,7 @@ From iris.proofmode Require Import base tactics classes.
 From iris.base_logic Require Export gen_heap ghost_map proph_map na_invariants.
 From iris.base_logic.lib Require Export fancy_updates.
 From iris.bi Require Export weakestpre.
-Require Export stack_common.
+Require Export stack_common is_empty.
 
 Set Implicit Arguments.
 Unset Strict Implicit.
@@ -22,105 +22,85 @@ Section stack.
 Section code.
 
 
-Definition pop :=
-  validate_stack 0 ++
+(*
+  pop: [i32] -> [i32]
+  locals declared: [i32]
+
+  Given a stack pointer, pop the top i32 value from the stack.
+
+  Implementation contains the is_empty check which results in a trap if the stack is empty. Otherwise, load the 
+  stack top pointer from the stack pointer address, retrieve the value to be popped, then decrement the stack
+  top pointer address by 4 and update it.
+  
+  Returns the popped value of type i32. Can trap only if the stack pointer is invalid or the stack is empty.
+
+  Parameters/Locals:
+  0 (input)     stack pointer
+  1             temporary variable storing the new address of the stack top pointer
+*)
+Definition pop_op :=
+  is_empty_op ++
   [
+    BI_if (Tf [] []) [BI_unreachable] [];
     BI_get_local 0 ;
     BI_load T_i32 None N.zero N.zero ;
-    i32const 4 ;
-    BI_binop T_i32 (Binop_i BOI_sub) ;
     BI_tee_local 1 ;
-  (* Check if stack is empty *)
-    BI_get_local 0 ;
-    BI_relop T_i32 (Relop_i ROI_eq) ;
-    BI_if (Tf [] []) [BI_unreachable] [] ;
-    BI_get_local 1 ; 
     BI_load T_i32 None N.zero N.zero ;
     BI_get_local 0 ;
     BI_get_local 1 ;
+    i32const 4 ;
+    BI_binop T_i32 (Binop_i BOI_sub) ;
     BI_store T_i32 None N.zero N.zero
   ].
+
+Definition pop :=
+  validate_stack 0 ++ validate_stack_bound 0 ++ pop_op.
 
 End code.
 
 Section specs.
 
-Lemma pop_not_empty (s: list i32) v E f:
-  (0 <= v <= Wasm_int.Int32.max_unsigned - 4 - S (length s) * 4 )%Z ->
-  f.(f_locs) !! 0 = Some (value_of_int v) ->
-  ↪[frame] f ⊢
-  WP [AI_basic (BI_const (value_of_int (v + S (length s) * 4))); AI_basic (BI_get_local 0);
-     AI_basic (BI_relop T_i32 (Relop_i ROI_eq)); AI_basic (BI_if (Tf [] []) [BI_unreachable] [])] @ E
-     {{ w, ⌜ w = immV [] ⌝ ∗ ↪[frame] f }}.
-Proof.
-  move => Hbounds Hlocs.
-  iIntros "Hf".
-  remember ((v + (S (length s) * 4))%Z) as x.
-  rewrite separate2.
-  iApply wp_seq.
-  instantiate (1 := λ w, (⌜ w = immV [value_of_int x; value_of_int v] ⌝ ∗ ↪[frame] f)%I).
-  iSplitR; first by iIntros "(%H & _)".
-  iSplitL "Hf".
-  { rewrite separate1. iApply wp_val_app => //.
-    iSplit => //.
-    { iIntros "!>".
-      by iIntros "(%H & _)".
-    }
-    by iApply (wp_get_local with "[] [Hf]") => //.
-  }
-  iIntros (w) "(-> & Hf)".
-
-  simpl.
-  rewrite separate3.
-  iApply wp_seq.
-  iSplitR; last iSplitL "Hf".
-  2: { iApply (wp_relop with "Hf") => //.
-       replace (app_relop _ _ _) with (false) => /=.
-       instantiate (1 := λ w, ⌜ w = immV [_]⌝%I) => //.
-       rewrite Wasm_int.Int32.eq_false => //.
-       move => Hcontra.
-       destruct Hbounds as [Hlb Hub].
-       unfold Wasm_int.Int32.max_unsigned in Hub.
-       apply Wasm_int.Int32.repr_inv in Hcontra => //=.
-       { subst.
-         assert ((S (length s) * 4 > 0)%Z) as Hlb2; by lias.
-       }
-       2: {
-         split; by lias.
-       }
-       { split; by lias. }
-     }
-  { by iIntros "(%H & _)". }
-
-  iIntros (w) "(-> & Hf)".
-  simpl.
-  iApply (wp_if_false with "Hf") => //.
-  iIntros "!> Hf".
-  replace ([AI_basic (BI_block (Tf [] []) [])]) with ([] ++ [AI_basic (BI_block (Tf [] []) [])]) => //.
-  iApply (wp_block with "Hf") => //.
-  iIntros "!> Hf".
-  by iApply (wp_label_value with "Hf").
-Qed.
-  
-Lemma spec_pop f0 n v (a : i32) s E:
+Lemma spec_pop_op f0 n v (a : i32) s E:
   ⊢ {{{ ⌜ f0.(f_inst).(inst_memory) !! 0 = Some n ⌝
          ∗ ⌜ f0.(f_locs) !! 0 = Some (value_of_int v) ⌝
          ∗ ⌜ length f0.(f_locs) >= 2 ⌝
          ∗ isStack v (a :: s) n
          ∗ ↪[frame] f0 }}}
-    to_e_list pop @ E
+    to_e_list pop_op @ E
     {{{ w, ⌜ w = immV [VAL_int32 a] ⌝ ∗
                       isStack v s n ∗
                       ∃ f1, ↪[frame] f1 ∗ ⌜ f_inst f0 = f_inst f1 ⌝ }}}.
 Proof.
   iIntros "!>" (Φ) "(%Hinst & %Hlocv & %Hlocs & Hstack & Hf) HΦ" => /=.
+  
   rewrite separate4.
   iApply wp_seq.
-  instantiate (1 := λ x,  (⌜ x = immV [] ⌝ ∗ isStack v (a :: s) n ∗ ↪[frame] f0)%I).
-  iSplitR; first by iIntros "(%H & _)".
-  iSplitL "Hstack Hf"; first by iApply (is_stack_valid with "[$Hstack $Hf]").
+  instantiate (1 := λ x,  (⌜x = immV [value_of_int 0]⌝ ∗ isStack v (a :: s) n ∗ ↪[frame] f0)%I).
+  iSplitR; last iSplitL "Hstack Hf".
+  2: { iApply (spec_is_empty_op with "[$Hstack $Hf]") => //.
+       iIntros (w) "H".
+       iDestruct "H" as (k) "(-> & Hstack & %Hk & Hf)".
+       iFrame "Hstack Hf".
+       by destruct Hk as [[-> ?] | [-> _]] => //.
+  }
+  { by iIntros "(%Habs & ?)". }
+  
   iIntros (w) "(-> & Hstack & Hf)".
   simpl.
+  rewrite separate2.
+  iApply wp_seq.
+  instantiate (1 := λ w, (⌜ w = immV [ ]⌝ ∗ ↪[frame] f0)%I).
+  iSplitR; first by iIntros "(%H & _)".
+  iSplitL "Hf".
+  iApply (wp_if_false with "Hf") => //.
+  { iIntros "!> Hf".
+    take_drop_app_rewrite 0.
+    iApply (wp_block with "Hf") => //.
+    iIntros "!> Hf /=".
+      by iApply (wp_label_value with "Hf").
+  }
+
+  iIntros (w) "(-> & Hf)" => /=.
   rewrite (separate1 (AI_basic _)).
   iApply wp_seq.
   instantiate (1 := λ x, (⌜ x = immV [value_of_int v] ⌝ ∗ ↪[frame] f0)%I).
@@ -128,12 +108,11 @@ Proof.
   iSplitL "Hf".
   - iApply (wp_get_local with "[] [$Hf]") => //=.
   - iIntros (w) "[-> Hf]".
-    unfold of_val, fmap, list_fmap.
     iSimpl.
     rewrite separate2.
     iApply wp_seq.
     iSplitR ; last first.
-    iDestruct "Hstack" as "(%Hdiv & %Hvub & %Hlen & Hv & Hs & Hrest)".
+    iDestruct "Hstack" as "(%Hdiv & %Hvb & %Hlen & Hv & Hs & Hrest)".
     iSplitR "HΦ".
   - iApply wp_load ; last first.
     iSplitL "Hs Hrest" ; last first.
@@ -141,72 +120,33 @@ Proof.
     iDestruct (i32_wms with "Hv") as "Hv" => //=.
     rewrite Wasm_int.Int32.Z_mod_modulus_eq.
     rewrite Z.mod_small; last first.
-    { unfold ffff0000 in Hvub; replace Wasm_int.Int32.modulus with 4294967296%Z; by lias. }
+    { unfold ffff0000 in Hvb; rewrite u32_modulus; by lias. }
     instantiate (1 := VAL_int32 _) => /=.
     rewrite N.add_0_r.
     done.
-    iNext.
-   
+    iNext.   
     by instantiate (1 := λ x, (⌜ x = immV _ ⌝ ∗ ( [∗ list] i↦w ∈ (a :: s)%SEQ, N.of_nat n
                                       ↦[i32][ Z.to_N
-                                                (v + 4 + length (a :: s) * 4 - 4 - 4 * i)] w) ∗ ( ∃ bs : seq.seq byte, ⌜Z.of_nat (length bs) = (two16 - 4 - length (a :: s) * 4)%Z⌝ ∗
-              N.of_nat n↦[wms][Z.to_N (v + 4 + length (a :: s) * 4)]bs))%I) ; iFrame.
+                                                (v + length (a :: s) * 4 - 4 * i)] w) ∗ ( ∃ bs : seq.seq byte, ⌜Z.of_nat (length bs) = (two16 - 4 - length (a :: s) * 4)%Z⌝ ∗
+              N.of_nat n↦[wms][Z.to_N (v + length (a :: s) * 4) + 4]bs))%I) ; iFrame.
     done.
     done.
+  2: { by iIntros "(((%Habs & _) & _) & _)". }
+    
   - iIntros (w) "[[(-> & Hs & Hrest) Hp] Hf]". 
     iAssert (isStack v (a :: s) n)%I with "[Hrest Hp Hs]" as "Hstack".
-    unfold isStack.
-    iFrame.
-    rewrite N.add_0_r.
-    simpl.
-    rewrite Wasm_int.Int32.Z_mod_modulus_eq.
-    rewrite Z.mod_small ; last first.
-    { unfold ffff0000 in Hvub; replace Wasm_int.Int32.modulus with 4294967296%Z; by lias. }
-    repeat iSplit => //=.
-    iApply i32_wms => //.
-  - unfold of_val, fmap, list_fmap.
-    iSimpl.
-    rewrite separate3.
-    iApply wp_seq.
-    instantiate (1 := λ x, (⌜ x = immV [value_of_int (v + S (length s) * 4)] ⌝ ∗
-                                       ↪[frame] f0)%I).
-    iSplitR ; first by iIntros "[%Habs _]".
-    iSplitL "Hf".
-  - iApply (wp_binop with "Hf") => //=.
-    iPureIntro.
-    unfold Wasm_int.Int32.isub, Wasm_int.Int32.sub.
-    unfold value_of_int.
-    repeat f_equal.
-    rewrite Wasm_int.Int32.unsigned_repr.
-    rewrite Wasm_int.Int32.unsigned_repr.
-    unfold value_of_int.
-    unfold Wasm_int.int_of_Z => //=.
-    remember (length s) as x.
-    rewrite - Heqx.
-    clear Heqx Hlen s.
-    replace (v + 4 + S x * 4 - 4)%Z with (v + S x * 4)%Z ; first done.
-    lia.
-    unfold Wasm_int.Int32.max_unsigned.
-    unfold Wasm_int.Int32.modulus.
-    unfold Wasm_int.Int32.wordsize.
-    unfold Integers.Wordsize_32.wordsize.
-    replace (two_power_nat 32) with 4294967296%Z ; last done.
-    lia.
-    simpl in Hlen.
-    unfold ffff0000 in Hvub.
-    unfold two14 in Hlen.
-    unfold Wasm_int.Int32.max_unsigned.
-    unfold Wasm_int.Int32.modulus.
-    unfold Wasm_int.Int32.wordsize.
-    unfold Integers.Wordsize_32.wordsize.
-    replace (two_power_nat 32) with 4294967296%Z ; last done.
-    remember (length s) as x.
-    rewrite - Heqx.
-    clear Heqx Hlen s.
-    lia.
-  - iIntros (w) "[-> Hf]".
-    unfold of_val, fmap, list_fmap.
-    iSimpl.
+    { unfold isStack.
+      iFrame.
+      rewrite N.add_0_r.
+      simpl.
+      rewrite Wasm_int.Int32.Z_mod_modulus_eq.
+      rewrite Z.mod_small ; last first.
+      { unfold ffff0000 in Hvb; rewrite u32_modulus; by lias. }
+      repeat iSplit => //=.
+      by iApply i32_wms => //.
+    }
+    
+  - iSimpl.
     rewrite separate2.
     iApply (wp_seq _ _ _ (λ x, (⌜ x = immV [value_of_int (v + S (length s) * 4)] ⌝
                                            ∗ ↪[frame] _)%I)).
@@ -218,43 +158,16 @@ Proof.
     iApply wp_val_app => //.
     iSplitR ; first by iIntros "!> [%Habs _]".
     iApply (wp_set_local with "[]Hf") => //.
+    
   - iIntros (w) "[-> Hf]".
     remember {| f_locs := set_nth (value_of_int (v + S (length s) * 4)) (f_locs f0) 1
                                   (value_of_int (v + S (length s) * 4)) ;
                 f_inst := f_inst f0 |} as f1.
     rewrite - Heqf1.
     iSimpl.
-
-    rewrite separate4.
-    iApply wp_seq.
-    iSplitR; last iSplitL "Hf".
-    2: { iApply (pop_not_empty with "Hf") => //.
-         rewrite Heqf1 => /=.
-         by destruct (f_locs f0) => //.
-       }
-    { by iIntros "(%H & _)". }
-    
-    iIntros (w) "(-> & Hf)".
-    simpl.
-
-    rewrite (separate1 (AI_basic (BI_get_local 1))).
-
-    iApply wp_seq.
-    iSplitR; last iSplitL "Hf".
-    2: { iApply (wp_get_local with "[] [Hf]") => //.
-         rewrite Heqf1 => /=.
-         by rewrite set_nth_read.
-         instantiate (1 := λ w, ⌜ w = immV [_] ⌝%I).
-         done.
-       }
-    { by iIntros "(%H & _)". }
-
-    iIntros (w) "(-> & Hf)".
-    simpl.
-    
     rewrite separate2.
     iApply wp_seq.
-    iDestruct "Hstack" as "(_ & _ & Hp & Hs & Hrest)".
+    iDestruct "Hstack" as "(_ & _ & _ & Hp & Hs & Hrest)".
     iSplitR ; last first.
     iSplitR "HΦ".
   - iApply wp_load ; last first.
@@ -267,31 +180,30 @@ Proof.
     rewrite Wasm_int.Int32.Z_mod_modulus_eq Z.mod_small.
     rewrite N.add_0_r Z.mul_0_r Z.sub_0_r.
     iDestruct "Ha" as "[Ha _]".
-    remember (length s) as x.
-    rewrite - Heqx.
-    clear Heqx Hlen s.
-    replace (v + 4 + S x * 4 - 4)%Z with (v + S x * 4)%Z.
     done.
-    lia.
-    unfold Wasm_int.Int32.max_unsigned in Hv. 
     remember (length s) as x.
     rewrite - Heqx.
-    clear Heqx Hlen s.
-    lia.
+    unfold ffff0000 in Hvb.
+    simpl in Hlen.
+    unfold two14 in Hlen.
+    rewrite - Heqx in Hlen.
+    rewrite u32_modulus.
+    by lias.
     by instantiate (1 := λ x, (⌜ x = immV _ ⌝ ∗ N.of_nat n
-                                          ↦[i32][ Z.to_N v] Wasm_int.Int32.repr (v + 4 + length ([a] ++ s)%list * 4) ∗
+                                          ↦[i32][ Z.to_N v] Wasm_int.Int32.repr (v + length ([a] ++ s)%list * 4) ∗
                                           ( ∃ bs : seq.seq byte,
                                               ⌜Z.of_nat (length bs) = (two16 - 4 - length ([a] ++ s)%list * 4)%Z⌝ ∗
-                                                                                                              N.of_nat n↦[wms][Z.to_N (v + 4 + length ([a] ++ s)%list * 4)]bs) ∗
+                                                                                                              N.of_nat n↦[wms][Z.to_N (v + length ([a] ++ s)%list * 4)+4]bs) ∗
                                           ([∗ list] k↦y ∈ s, N.of_nat n
                            ↦[i32][ Z.to_N
-                                     (v + 4 + length ([a] ++ s)%list * 4 - 4 -
+                                     (v + length ([a] ++ s)%list * 4 -
                                         4 * (length [a] + k)%nat)] y))%I) ; iFrame.
     subst f1.
     done.
     done.
+  2: { by iIntros "(((%Habs & _) & _) & _)". }
+    
   - iIntros (w) "[[(-> & Hp & Hrest & Hs) Ha] Hf]".
-    unfold of_val, fmap, list_fmap.
     iSimpl.
     rewrite separate2.
     iApply wp_seq.
@@ -304,7 +216,8 @@ Proof.
     subst.
     iApply (wp_get_local with "[] [$Hf]") => //=.
     unfold set_nth.
-    destruct (f_locs f0) => //=.
+    by destruct (f_locs f0) => //=.
+    
   - iIntros (w) "[-> Hf]".
     unfold of_val, fmap, list_fmap.
     iSimpl.
@@ -321,8 +234,38 @@ Proof.
     iApply (wp_get_local with "[] [$Hf]") => //=.
     subst f1 => //=.
     by rewrite set_nth_read.
+      
   - iIntros (w) "[-> Hf]".
-    unfold of_val, fmap, list_fmap.
+    iSimpl.
+    rewrite separate5.
+    iApply wp_seq.
+    instantiate (1 := λ x, (⌜ x = immV [VAL_int32 a ; value_of_int v ;
+                                        value_of_int (v + (length s) * 4)] ⌝ ∗
+                                       ↪[frame] f1)%I).
+    iSplitR ; first by iIntros "[%Habs _]".
+    iSplitL "Hf".
+    rewrite (separate2 (AI_basic _)).
+    iApply wp_val_app => //.
+    iSplitR ; first by iIntros "!> [%Habs _]".
+    iApply (wp_binop with "Hf") => //.
+    simpl.
+    iModIntro.
+    iPureIntro.
+    unfold value_of_int.
+    repeat f_equal.
+    unfold Wasm_int.Int32.isub, Wasm_int.Int32.sub => /=.
+    f_equal.
+    rewrite Wasm_int.Int32.Z_mod_modulus_eq.
+    remember (length s) as x.
+    rewrite - Heqx.
+    rewrite Z.mod_small; first by lias.
+    unfold ffff0000 in Hvb.
+    unfold two14 in Hlen. simpl in Hlen.
+    rewrite - Heqx in Hlen.
+    rewrite u32_modulus.
+    by lias.
+
+  - iIntros (w) "[-> Hf]".
     iSimpl.
     iApply wp_wand_r.
     iSplitL "Hp Hf".
@@ -330,19 +273,19 @@ Proof.
     iApply wp_val_app => //.
     instantiate (1 := λ x, ((⌜ x = immV [VAL_int32 a] ⌝ ∗
                                        N.of_nat n↦[wms][Wasm_int.N_of_uint i32m
-                                                                           (Wasm_int.int_of_Z i32m v) + N.zero]bits (value_of_int (v + S (length s) * 4))) ∗
-                                                                                                                                                           ↪[frame] f1)%I).
+                                                                           (Wasm_int.int_of_Z i32m v) + N.zero]bits (value_of_int (v + (length s) * 4))) ∗ ↪[frame] f1)%I).
     iSplit ; first by iIntros "!> [[%Habs _] _]".
     iApply wp_store => //.
-    instantiate (1 := bits (value_of_int (v + 4 + length (a :: s) * 4))) => //=.
+    instantiate (1 := bits (value_of_int (v + length (a :: s) * 4))) => //=.
     subst f1 => //=.
     iSimpl.
     rewrite Wasm_int.Int32.Z_mod_modulus_eq.
-    rewrite Z.mod_small ; last by unfold Wasm_int.Int32.max_unsigned in Hv ; lia.
+    rewrite Z.mod_small; last by unfold ffff0000 in Hvb; rewrite u32_modulus; lias.
     rewrite N.add_0_r.
     iFrame.
     iSplitR => //=.
     iDestruct (i32_wms with "Hp") as "Hp" => //.
+    
   - iIntros (w) "[[-> Hp] Hf]".
     iApply "HΦ".
     iSplitR => //.
@@ -352,29 +295,25 @@ Proof.
     repeat iSplit => //.
     iPureIntro.
     remember (length s) as x. rewrite - Heqx in Hlen ; clear Heqx s ; lia.
-    iFrame.
     iSplitL "Hp".
   - simpl. rewrite Wasm_int.Int32.Z_mod_modulus_eq.
-    rewrite Z.mod_small ; last by unfold Wasm_int.Int32.max_unsigned in Hv ; lia.
+    rewrite Z.mod_small; last by unfold ffff0000 in Hvb; rewrite u32_modulus; lias.
     rewrite N.add_0_r.
     iApply i32_wms => //.
-    unfold value_of_int => /=.
-    remember (length s) as x. rewrite - Heqx ; clear Heqx Hlen s.
+  - unfold value_of_int => /=.
+    remember (length s) as x. rewrite - Heqx.
     replace (v + S (x) * 4)%Z with (v + 4 + x * 4)%Z ; last lia.
-    done.
-  - iDestruct "Hrest" as (bs) "[%Hbs Hrest]".
     iSplitL "Hs".
     iApply (big_sepL_impl with "Hs").
     iIntros "!>" (k y) "% H".
     simpl.
-    remember (length s) as x ; rewrite - Heqx ; clear Heqx Hbs H Hlen s.
-    replace ( v + 4 + S x * 4 - 4 - 4 * S k)%Z with
-      (v + 4 + x * 4 - 4 - 4 * k)%Z.
+    replace ( v + 4 + x * 4 - 4 * S k)%Z with
+      (v + x * 4 - 4 * k)%Z.
     done.
     lia.
+  - iDestruct "Hrest" as (bs) "(%Hbs & Hrest)".
     iExists (serialise_i32 a ++ bs).
-    iFrame.
-    iSplitR.
+    iSplit.
     iPureIntro.
     rewrite app_length.
     simpl in Hbs.
@@ -385,35 +324,70 @@ Proof.
     destruct l ; last done.
     simpl.
     lia.
-    unfold mem_block_at_pos.
+  - unfold mem_block_at_pos.
     rewrite big_sepL_app.
     iSplitL "Ha".
     iApply (big_sepL_impl with "Ha").
-    iIntros "!>" (k x) "%Hbits H".
+    iIntros "!>" (k ?) "%Hbits H".
     rewrite of_nat_to_nat_plus.
     rewrite N.add_0_r.
     rewrite of_nat_to_nat_plus.
     unfold Wasm_int.N_of_uint => //=.
     rewrite Wasm_int.Int32.Z_mod_modulus_eq.
-    rewrite Z.mod_small ; last by unfold Wasm_int.Int32.max_unsigned in Hv ; remember (length s) as y ; rewrite - Heqy ; clear Heqy Hbs Hlen s ; lia.
-    remember (length s) as y ; rewrite - Heqy ; clear Heqy Hbs Hlen s.
-    replace (v + S (y) * 4)%Z with (v + 4 + y * 4)%Z ; last lia.
+    rewrite Z.mod_small ; last first.
+    { rewrite u32_modulus.
+      rewrite -Heqx in Hlen.
+      unfold ffff0000 in Hvb.
+      unfold two14 in Hlen.
+      by lias.
+    }
+    replace (Z.to_N (v + 4 + x * 4)%Z) with ((Z.to_N (v + x * 4)) + 4)%N ; last lia.
     done.
-    iApply (big_sepL_impl with "Hrest").
-    iIntros "!>" (k x) "%Hbits H".
+    
+  - iApply (big_sepL_impl with "Hrest").
+    iIntros "!>" (k ?) "%Hbits H".
     repeat rewrite of_nat_to_nat_plus.
     remember (serialise_i32 a) as l.
     repeat (destruct l => //).
     simpl.
-    remember (length s) as y ; rewrite - Heqy ; clear Heqy Hbs Hlen s.
-    replace (Z.to_N (v + 4 + S y * 4) + N.of_nat k)%N
-      with (Z.to_N (v + 4 + y * 4) + N.of_nat (4+k))%N ; first done.
-    simpl.
-    lia.
+    replace (Z.to_N (v + 4 + x * 4) + 4 + N.of_nat k)%N
+      with (Z.to_N (v + x * 4) + 4 + N.of_nat (4+k))%N ; last lias.
+    done.
     iExists _ ; by subst ; iFrame.
-    all : try by iIntros "[[[% _] _] _]".
 Qed.    
     
+Lemma spec_pop f0 n v (a : i32) s E:
+  ⊢ {{{ ⌜ f0.(f_inst).(inst_memory) !! 0 = Some n ⌝
+         ∗ ⌜ f0.(f_locs) !! 0 = Some (value_of_int v) ⌝
+         ∗ ⌜ length f0.(f_locs) >= 2 ⌝
+         ∗ isStack v (a :: s) n
+         ∗ ↪[frame] f0 }}}
+    to_e_list pop @ E
+    {{{ w, ⌜ w = immV [VAL_int32 a] ⌝ ∗
+                      isStack v s n ∗
+                      ∃ f1, ↪[frame] f1 ∗ ⌜ f_inst f0 = f_inst f1 ⌝ }}}.
+Proof.
+  iIntros "!>" (Φ) "(%Hinst & %Hlocv & %Hlocs & Hstack & Hf) HΦ" => /=.
+  
+  rewrite separate4.
+  iApply wp_seq.
+  instantiate (1 := λ x,  (⌜ x = immV [] ⌝ ∗ isStack v _ n ∗ ↪[frame] f0)%I).
+  iSplitR; first by iIntros "(%H & _)".
+  iSplitL "Hstack Hf"; first by iApply (is_stack_valid with "[$Hstack $Hf]").
+  
+  iIntros (w) "(-> & Hstack & Hf) /=".
+  rewrite separate3.
+  iApply wp_seq.
+  instantiate (1 := λ x,  (⌜ x = immV [] ⌝ ∗ isStack v _ n ∗ ↪[frame] f0)%I).
+  iSplitR; first by iIntros "(%H & _)".
+  iSplitL "Hstack Hf"; first by iApply (is_stack_bound_valid with "[$Hstack $Hf]").
+  
+  iIntros (w) "(-> & Hstack & Hf) /=".
+  iApply (spec_pop_op with "[$Hf $Hstack] [$]").
+  auto.
+Qed.
+
+
 End specs.
 
 
